Squashed commit the interpreter branch, containing the following commits:
commit 4cbef8039851ae5b776574eab84f0903bd383870
Author: Jean-Marie Madiot <jean-marie.madiot@inria.fr>
Date:   Mon May 26 18:40:46 2025 +0200

    clean up run.v

commit 9e08dfd15ed7cddfc731526d7ef8b909ef2a84ce
Author: Jean-Marie Madiot <jean-marie.madiot@inria.fr>
Date:   Mon May 26 17:05:17 2025 +0200

    some tests

commit 7eba1df201293fe30953a2c7c9d93533356011d2
Author: Jean-Marie Madiot <jean-marie.madiot@inria.fr>
Date:   Mon May 26 16:52:54 2025 +0200

    merged eval and eval_strat

commit 70a17d930eb495396c57841ee4a4cc1fa8955282
Author: Jean-Marie Madiot <jean-marie.madiot@inria.fr>
Date:   Mon May 26 16:48:38 2025 +0200

    tuple evaluation order

commit 27c9eead6b81e0d48fb3156eda6f7717126d6d3f
Author: Jean-Marie Madiot <jean-marie.madiot@inria.fr>
Date:   Mon May 26 16:23:06 2025 +0200

    strategy option for for-boundaries

commit 32034d627243a353d490ee06737dd28256bf32f9
Author: Jean-Marie Madiot <jean-marie.madiot@inria.fr>
Date:   Mon May 26 13:36:19 2025 +0200

    wrapping eval.v in a functor: almost seamless

commit 7b602e10707fa42574858f205af722de3b2985e4
Author: Jean-Marie Madiot <jean-marie.madiot@inria.fr>
Date:   Sun May 25 21:12:54 2025 +0200

    strategies now modules instead of records

commit 68cfee34cde472b018a72748080f239eef271a5e
Author: Jean-Marie Madiot <jean-marie.madiot@inria.fr>
Date:   Sun May 25 18:44:23 2025 +0200

    several strategy renamings

commit 294ef6eb058e453c1c6da6f59a50fcbf3ddb0ed7
Author: Jean-Marie Madiot <jean-marie.madiot@inria.fr>
Date:   Sun May 25 17:50:23 2025 +0200

    renaming options->strategy

commit 9d6adc472cdad47a184a4482405281eddc556b34
Author: Jean-Marie Madiot <jean-marie.madiot@inria.fr>
Date:   Thu May 22 17:49:07 2025 +0200

    bug fix: VData argument length mismatch allowed if constructors are different

commit dd5d9d4b7ff26e7b44e2112c1be420e746d9ff19
Author: Jean-Marie Madiot <jean-marie.madiot@inria.fr>
Date:   Thu May 22 17:42:29 2025 +0200

    micro: Crash now has a string argument

commit c7cf398b51a836b9fea82e1ff3fc1fc40e11c5f9
Author: Jean-Marie Madiot <jean-marie.madiot@inria.fr>
Date:   Thu May 22 15:26:37 2025 +0200

    internal libraries rather than packages

commit ff1abd02167d56994e7a838c5e2585d65d3cc39f
Author: Jean-Marie Madiot <jean-marie.madiot@inria.fr>
Date:   Thu May 22 15:09:26 2025 +0200

    oStdlib->Stdlib

commit 2697ffb1b95dbe12d7781d93c914f85b680397b2
Author: Jean-Marie Madiot <jean-marie.madiot@inria.fr>
Date:   Thu May 22 14:43:02 2025 +0200

    moving extracted file to dedicated package

commit 7d8c13a138c273e26a15d3d7a13beadc6fb7e93e
Author: Jean-Marie Madiot <jean-marie.madiot@inria.fr>
Date:   Thu May 22 14:11:05 2025 +0200

    removed symlinks, moved translator lib to a subdir in interp

commit bd4adda837d0e0e01dec18f3a1dd1dc6bb3cff98
Author: Jean-Marie Madiot <jean-marie.madiot@inria.fr>
Date:   Thu May 22 13:59:14 2025 +0200

    suppress unused arg (necessary to fit compiler-libs) warning

commit 0b1ce27401171604b1e5e213e2aab4f47c742e02
Author: Jean-Marie Madiot <jean-marie.madiot@inria.fr>
Date:   Thu May 22 13:58:05 2025 +0200

    moved Read module to interp, leaving only symlinked modules in lib

commit a4be2a476fca9234f06056db7b3553cb54c628f6
Author: Jean-Marie Madiot <jean-marie.madiot@inria.fr>
Date:   Thu May 22 13:35:17 2025 +0200

    interpreter

commit 86f9982caf5273fcee6fcf23ec4f3095654c645a
Author: Jean-Marie Madiot <jean-marie.madiot@inria.fr>
Date:   Thu May 22 11:36:19 2025 +0200

    avoid running the osiris translator on the interpreter

commit 223ccfe025de5c27f65ceb342b41630cae86ce39
Author: Jean-Marie Madiot <jean-marie.madiot@inria.fr>
Date:   Thu May 22 11:34:32 2025 +0200

    git clean->dune clean

commit d16bab48055e2a775875216f8bfb1b6dd123b74a
Author: Jean-Marie Madiot <jean-marie.madiot@inria.fr>
Date:   Thu May 22 11:32:14 2025 +0200

    rename Stdlib->oStdlib to avoid conflicts

commit 101fe3c5cfaa1736a7fee00f5fe1c7d6e09e4f53
Author: Jean-Marie Madiot <jean-marie.madiot@inria.fr>
Date:   Fri May 16 17:24:26 2025 +0200

    Settings is now loaded by Main, not by Translate

coq-osiris/interp/E2O.mli
@@ -1,0 +1,50 @@
+open Extracted.BinNums
+open Extracted.Datatypes
+
+(** Conversions from extracted (E) to manually-defined-in-OCaml types (O) *)
+
+(* Convention: [ty] is the name of the function converting type [ty], so as to
+   have [E2O.ty : E.ty -> O.ty] *)
+
+(* There is a lot of shadowing involved, so we sometimes use [Stdlib.Module.t]
+   instead of the corresponding predefined type such as [string] or [list] *)
+
+(* [Stdlib] lets us reference OCaml's standard library. Osiris's standard
+   library has a different module name to prevent shadowing. *)
+
+val z : coq_Z -> int
+val nat : nat -> int
+val list : ('a -> 'b) -> 'a list -> 'b Stdlib.List.t
+val prod : ('a1 -> 'b1) -> ('a2 -> 'b2) -> ('a1 * 'a2) -> ('b1 * 'b2)
+val string : Extracted.String.string -> Stdlib.String.t
+
+module O = Translatorlib.Syntax
+module E = Extracted.Syntax (* from syntax.ml, extracted from syntax.v *)
+
+(* Enumeration of [val ty : E.ty -> O.ty] for each syntax type [ty] *)
+
+val var          : E.var                -> O.var
+val name         : E.name               -> O.name
+val path         : E.path               -> O.path
+val data         : E.data               -> O.data
+val field        : E.field              -> O.field
+val pat          : E.pat                -> O.pat
+val cpat         : E.cpat               -> O.cpat
+val pats         : E.pat list           -> O.pats
+val fpats        : E.(field * pat) list -> O.fpats
+val coercion     : E.coercion           -> O.coercion
+val fcoercions   : E.fcoercion list     -> O.fcoercions
+val expr         : E.expr               -> O.expr
+val exprs        : E.expr list          -> O.exprs
+val fexpr        : E.fexpr              -> O.fexpr
+val fexprs       : E.fexpr list         -> O.fexprs
+val branch       : E.branch             -> O.branch
+val branches     : E.branch list        -> O.branches
+val binding      : E.binding            -> O.binding
+val bindings     : E.binding list       -> O.bindings
+val rec_binding  : E.rec_binding        -> O.rec_binding
+val rec_bindings : E.rec_binding list   -> O.rec_bindings
+val anonfun      : E.anonfun            -> O.anonfun
+val mexpr        : E.mexpr              -> O.mexpr
+val sitems       : E.sitem list         -> O.sitems
+val sitem        : E.sitem              -> O.sitem
