coq-osiris/interp/Read.mli
@@ -1,0 +1,1 @@
+val typedtree_of_filename : string -> Typedtree.implementation
