coq-osiris/interp/interp.ml
@@ -1,0 +1,246 @@
+open Printf
+
+(* Extracted modules *)
+open Extracted.Syntax
+open Extracted.Run
+
+(* OCaml's stdlib; shadows some extracted modules such as List and String *)
+open Stdlib
+
+
+(* Parsing commandline arguments *)
+
+let noorder = ref false
+let debug = ref false
+let detcheck = ref false
+let random = ref false
+let show_ast = ref false
+let verbose = ref false
+let warnings = ref true
+
+let filename = ref None
+
+let usage_msg = sprintf "Usage: %s <options> <file.ml>" Sys.argv.(0)
+
+let () =
+  let open Arg in
+  parse
+    (align [
+        "--noorder", Set noorder, " Evaluation order is less constrained, typically used with --random or --detcheck (default: compiler evaluation order)";
+        "--debug", Set debug, " (passed to Osiris translator)";
+        "--detcheck", Set detcheck, " Determinism check: do no print, but compare output traces, prints the first difference found";
+        "--no-warnings", Clear warnings, " Disable warnings (default: enabled)";
+        "--show-ast", Set show_ast, " Show AST of typed tree (default: disabled)";
+        "--random", Unit (fun () -> random := true; Random.self_init ()), " When faced with a choice during evaluation, choose a random branch (default: choose the first option)";
+        "--verbose", Set verbose, " Displays intermediate evaluation steps";
+        "--warnings", Set warnings, " Enable warnings (default: enabled)"])
+    (fun anon ->
+       if !filename <> None || not (Filename.check_suffix anon "ml") then
+         raise (Arg.Bad ("Error at argument: " ^ anon));
+       filename := Some anon)
+    usage_msg;
+  if !random && !detcheck then
+    fprintf stderr "Warning: option --random unused if --detcheck is set.\n%!"
+
+let filename =
+  match !filename with
+  | Some s -> s
+  | None -> fprintf stderr "%s\n%!" usage_msg; exit 0
+
+(* Use Osiris's [Translate] module with a dummy [Settings] module *)
+module Translate =
+  Translatorlib.Translate.Make(struct
+    let warnings = !warnings
+    let debug format = (if !debug then fprintf else ifprintf) stderr format
+  end)
+
+
+(** Handling the special I/O effect allocated at [io_loc] *)
+
+type 'a iostep =
+  | StepIn_int of (int -> 'a)
+  | StepIn_str of (string -> 'a)
+  | StepOut of string * 'a
+
+(** Interpret interactively an [iostep] by actually printing to standard output
+    or reading from standard input *)
+let interactive_io (s : 'a iostep) : 'a =
+  match s with
+  | StepIn_int f -> f (read_int ())
+  | StepIn_str f -> f (read_line ())
+  | StepOut (o, a) -> printf "%s%!" o; a
+
+(** Convert argument list [args] (e.g. [["print_int"; 3]] or [["read_int"; ()]])
+    passed to the I/O effect into a ['a iostep], through a continuation [k]
+    taking the returned value as argument (respectively [VUnit] for [print_int],
+    or say [Vint 4] for [read_int]) *)
+let iostep_from_args (args : coq_val list) (k : coq_val -> 'a) : 'a iostep =
+  let err =
+    Failure
+      (sprintf "I/O error with argument list [%s]"
+         (String.concat ";" List.(map E2O.string (map string_of_val args)))) in
+  let name, arg =
+    match [@warning "-4"] args with
+    | [VString name; arg] -> E2O.string name, arg
+    | _ -> raise err in
+  let unit = VData (O2E.string "()", []) in
+  match [@warning "-4"] name, arg with
+  | "print_int", VInt n -> StepOut (string_of_int (E2O.z n), k unit)
+  | "print_string", VString s -> StepOut (E2O.string s, k unit)
+  | "print_endline", VString s -> StepOut (E2O.string s ^ "\n", k unit)
+  | "print_newline", u when u = unit -> StepOut ("\n", k unit)
+  | "read_int", u when u = unit -> StepIn_int (fun n -> k (VInt (O2E.z n)))
+  | "read_line", u when u = unit -> StepIn_str (fun s -> k (VString (O2E.string s)))
+  | _ -> raise err
+
+(* Some stepping functions below take a stepping function [step], taking a
+   [config] and returning a [step_result] *)
+
+(** Stepping function that detects special I/O effects, those at location
+    [io_loc], out of the results of the [step] function. Returns an [iostep]
+    tagged with [`IO] or the normal output of [step], tagged with [`Silent]. *)
+let io_step step cfg =
+  match step cfg with
+  | Step l -> `Silent (Step l)
+  | Final f ->
+    match f with
+    | FRet _ | FCrash _ | FThrow _ -> `Silent (Final f)
+    | FPerform (eff, k) ->
+      match [@warning "-4"] eff with
+      | VXData(loc, args) when loc = io_loc ->
+        `IO (iostep_from_args args (fun v -> (fst cfg, k (O2Ret v))))
+      | _ -> `Silent (Final f)
+
+(** Stepping function that forbids reads and discards final states, used for
+    collecting outputs. Returns a list of configuration tagged with [`Silent],
+    or a pair of the output string and the continuation configuration, tagged
+    with [`Output]. *)
+let output_step step cfg =
+  match io_step step cfg with
+  | `Silent (Step l) -> `Silent l
+  | `Silent (Final _) -> `Silent []
+  | `IO io ->
+    match io with
+    | StepOut (s, cfg) -> `Output (s, cfg)
+    | StepIn_int _ | StepIn_str _ -> failwith "determinism check forbids reads"
+
+(** [determinism_check step cfg] checks that all output traces that [cfg] can
+    generate are all the same, in which case [None] is returned. Otherwise,
+    [Some (trace, o1, o2)] is returned where [trace] is a common prefix and [o1]
+    and [o2] is the first difference. *)
+
+(* It does so by calling [det_check_silence], that evaluates configurations in
+   the list [active] until one performs an output event [o], in which case its
+   continuation becomes [paused], and the other configurations become [active]
+   and [det_check_output] checks that they all also output [o], it which case it
+   calls [det_check_silence] again. If a configuration outputs something else,
+   evaluation stops and the difference is returned. *)
+
+let rec det_check_silence step trace active =
+  match active with
+  | [] -> None
+  | cfg :: active ->
+    match output_step step cfg with
+    | `Silent cfgs -> det_check_silence step trace (cfgs @ active)
+    | `Output (o, cfg) -> det_check_output step (o :: trace) o [cfg] active
+and det_check_output step trace output paused active =
+  match active with
+  | [] -> det_check_silence step trace paused
+  | cfg :: active ->
+    match output_step step cfg with
+    | `Silent cfgs -> det_check_output step trace output paused (cfgs @ active)
+    | `Output (o, cfg') ->
+      if o <> output then
+        Some (List.rev trace, output, o)
+      else
+        det_check_output step trace output (cfg' :: paused) active
+
+let determinism_check step cfg = det_check_silence step [] [cfg]
+
+
+(** Interactive run *)
+
+let interactive_run step cfg =
+  (* How to choose which branch when encountering a non-confluent step *)
+  let choose =
+    if !random then
+      fun l -> List.(nth l (Random.int (length l)))
+    else
+      List.hd
+  in
+
+  (* Collect some stats *)
+  let steps = ref 0 in
+  let choices = ref 0 in
+
+  let t = Sys.time () in
+  let print_info (store, micro) =
+    printf "Stats: %d steps, %d choices in branching, %f seconds elapsed\n"
+      !steps
+      !choices
+      (Sys.time () -. t);
+    printf "Store: %s\n" (E2O.string (string_of_store store));
+    printf "Micro: %s\n" (E2O.string (string_of_microvx micro))
+  in
+
+  (* Run io step function until termination *)
+  let rec run cfg =
+    incr steps;
+    if !verbose then
+      printf "Step: %s\n%!" (E2O.string (string_of_microvx (snd cfg)));
+    match io_step step cfg with
+    | `IO io -> run (interactive_io io)
+    | `Silent r ->
+      match r with
+      | Final (FRet _) -> cfg
+      | Final (FCrash s) -> fprintf stderr "Crash: %s\n%!" (E2O.string s); exit 1
+      | Final (FThrow _) -> fprintf stderr "Unhandled exception\n%!"; exit 1
+      | Final (FPerform (_, _)) -> fprintf stderr "Unhandled effect\n%!"; exit 1
+      | Step l ->
+        match l with
+        | [] -> failwith "Step []"
+        | [cfg'] -> run cfg'
+        | _ :: _ :: _ -> incr choices; run (choose l)
+  in
+  let cfg = run cfg in
+  if !verbose then (print_newline(); print_info cfg)
+
+
+let () =
+  (* Parse file passed as first argument as an OCaml typedtree *)
+  let typedtree = Read.typedtree_of_filename filename in
+
+  (* Translate it into an osiris AST, then into extracted syntax *)
+  let mexpr : Translatorlib.Syntax.mexpr =
+    Translate.unit (Some filename) typedtree.structure in
+  if !show_ast then
+    fprintf stdout "Typed tree:\n%s\n\n" (Translatorlib.Syntax.show_mexpr mexpr);
+  let mexpr : Extracted.Syntax.mexpr = O2E.mexpr mexpr in
+
+  flush_all ();
+
+  (* Choose evaluation options between "usual" and "liberal" *)
+  let strat =
+    Extracted.Strategy.(
+      if !noorder then
+        (module LiberalStrategy : Strategy)
+      else
+        (module UsualStrategy : Strategy))
+  in
+
+  let module R = Extracted.Run.RunF(val strat) in
+  let module E = Extracted.Eval.EvalF(val strat) in
+
+  (* Make [mexpr] into a configuration (store, micro) *)
+  let env = io_env @ effect_stdlib_env in
+  let store = io_store in
+  let config = (store, E.eval_mexpr env mexpr) in
+
+  if !detcheck then
+    match determinism_check R.step config with
+    | Some (history, out1, out2) ->
+      printf "Different outputs detected: '%s' vs '%s'\n" out1 out2;
+      printf "common output prefix: [%s]\n%!" (String.concat "; " history)
+    | None -> printf "Detected no non-deterministic behavior.\n%!"
+  else
+    interactive_run R.step config
