osiris/src/Translate.mli
@@ -1,4 +1,15 @@
-(**[unit osource u] translates the OCaml typed AST [u], which represents a
-   compilation unit, to an Osiris AST. The optional argument [osource] is
-   the content of the OCaml source file. *)
-val unit : string option -> Typedtree.structure -> Syntax.mexpr
+(** [Translate] is a functor taking a settings module as a parameter. When
+    producing the [Main] executable, it will be instantiated by the module
+    [Settings], which parses the command line. This lets the interpreter use
+    [Translate] without triggering the side effects in [Settings]. *)
+module Make (_ : sig
+  val warnings : bool
+  val debug : ('a, out_channel, unit) format -> 'a
+end) : sig
+
+  (** [unit osource u] translates the OCaml typed AST [u], which represents a
+      compilation unit, to an Osiris AST. The optional argument [osource] is the
+      content of the OCaml source file. *)
+  val unit : string option -> Typedtree.structure -> Syntax.mexpr
+
+end
