tests/eff01.ml
@@ -1,0 +1,164 @@
+(* Examples from https://ocaml.org/manual/effects.html  *)
+
+open Effect
+open Effect.Deep
+
+type _ Effect.t += Xchg: int -> int t
+
+let comp1 () = perform (Xchg 0) + perform (Xchg 1)
+
+let () = print_int (
+    try comp1 () with
+      effect (Xchg n), k -> continue k (n+1)
+  )
+
+type 'a status =
+  Complete of 'a
+| Suspended of {msg: int; cont: (int, 'a status) continuation}
+
+let step (f : unit -> 'a) () : 'a status =
+  match f () with
+  | v -> Complete v
+  | effect (Xchg msg), cont -> Suspended {msg; cont}
+
+let rec run_both a b =
+  match a (), b () with
+  | Complete va, Complete vb -> (va, vb)
+  | Suspended {msg = m1; cont = k1},
+    Suspended {msg = m2; cont = k2} ->
+      run_both (fun () -> continue k1 m2)
+               (fun () -> continue k2 m1)
+  | _ -> failwith "Improper synchronization"
+
+
+let comp2 () = perform (Xchg 21) * perform (Xchg 21)
+
+let () =
+  let (a, b) = run_both (step comp1) (step comp2) in
+  assert (a = 42);
+  assert (b = 0);
+  print_int (a * 100 + b)
+
+let () = print_newline ()
+
+type _ Effect.t += Fork : (unit -> unit) -> unit t
+                 | Yield : unit t
+let fork f = perform (Fork f)
+let yield () = perform Yield
+let xchg v = perform (Xchg v)
+
+module Queue = struct
+  type 'a t = 'a list ref
+  let create () = ref []
+  let push x q = q := x :: !q
+  let pop q = match !q with [] -> invalid_arg "pop" | x :: l -> q := l; x
+  let is_empty q = !q = []
+end
+
+
+(* A concurrent round-robin scheduler *)
+let run (main : unit -> unit) : unit =
+  let exchanger : (int * (int, unit) continuation) option ref =
+    ref None (* waiting exchanger *)
+  in
+  let run_q = Queue.create () in (* scheduler queue *)
+  let enqueue k v =
+    let task () = continue k v in
+    Queue.push task run_q
+  in
+  let dequeue () =
+    if Queue.is_empty run_q then () (* done *)
+    else begin
+      let task = Queue.pop run_q in
+      task ()
+    end
+  in
+  let rec spawn (f : unit -> unit) : unit =
+    match f () with
+    | () -> dequeue ()
+    | exception e ->
+        print_endline "Printexc.to_string e";
+        dequeue ()
+    | effect Yield, k -> enqueue k (); dequeue ()
+    | effect (Fork f), k -> enqueue k (); spawn f
+    | effect (Xchg n), k ->
+        begin match !exchanger with
+        | Some (n', k') -> exchanger := None; enqueue k' n; continue k n'
+        | None -> exchanger := Some (n, k); dequeue ()
+        end
+  in
+  spawn main
+
+let _ = run (fun _ ->
+  fork (fun _ ->
+    print_endline "[t1] Sending 0";
+    let v = xchg 0 in
+    print_string "[t1] received "; print_int v; print_newline ());
+  fork (fun _ ->
+    print_endline "[t2] Sending 1";
+    let v = xchg 1 in
+    print_string "[t2] received "; print_int v; print_newline ()))
+
+module Seq = struct
+  type +'a node =  Nil | Cons of 'a * 'a t
+  and 'a t = unit -> 'a node
+  let to_dispenser xs =
+    let s = ref xs in
+    fun () ->
+      match (!s)() with
+      | Nil ->
+        None
+      | Cons (x, xs) ->
+        s := xs;
+        Some x
+end
+
+let invert (type a) (iter : (a -> unit) -> unit) : a Seq.t =
+  let module M = struct
+    type _ Effect.t += Yield : a -> unit t
+  end in
+  let yield v = perform (M.Yield v) in
+  fun () -> match iter yield with
+  | () -> Seq.Nil
+  | effect M.Yield v, k -> Seq.Cons (v, fun x -> continue k x)
+
+
+let rec map f = function [] -> [] | x :: l -> f x :: map f l
+let rec sum = function [] -> 0 | x :: l -> x + sum l
+let rec seq a b = if a > b then [] else a :: seq (a + 1) b
+let rec iter f l = match l with [] -> () | x :: l -> f x; iter f l
+let rec hash = function [] -> 0 | x :: l -> x + 7 * hash l
+
+let lst_iter f = iter f [1;2;3]
+let () = lst_iter (fun i -> print_int i)
+let s = invert lst_iter
+let next = Seq.to_dispenser s
+
+let print_int_option o =
+  match o with
+  | None -> print_string "None"
+  | Some n -> print_string "Some "; print_int n
+
+let () =
+  print_int_option (next ());
+  print_int_option (next ());
+  print_int_option (next ());
+  print_int_option (next ());
+  ()
+
+
+
+type _ Effect.t += E : int t
+                 | F : string t
+
+let foo () = perform F
+
+let bar () =
+  try foo () with
+  | effect E, k -> failwith "impossible"
+
+let baz () =
+  try bar () with
+  | effect F, k -> continue k "Hello, world!"
+
+let () = print_endline (baz ())
