tests/eff03.ml
@@ -1,0 +1,12 @@
+open Effect
+open Effect.Deep
+
+type _ Effect.t += E : int -> int Effect.t
+
+let x =
+  let r = ref 1 in
+  try
+    perform (E (2 * perform (E 1)))
+    with effect E n, k -> r := !r + 1; continue k (n + !r)
+
+let () = print_int x
