tests/exn01.ml
@@ -1,0 +1,40 @@
+let x =
+  let r = ref 1 in
+  try
+    1 / !r
+  with
+    _ -> 42
+
+let () = assert (x = 1)
+
+let () = print_int x
+
+exception A
+exception B
+
+let () =
+  print_int (try raise A + 2 with A -> 4);
+  print_int (try (if true then raise A; 3) with A -> 4);
+  print_int (try (if false then raise A; 3) with A -> 4);
+  ()
+
+
+
+
+let rec map f = function [] -> [] | x :: l -> f x :: map f l
+let rec sum = function [] -> 0 | x :: l -> x + sum l
+let rec seq a b = if a > b then [] else a :: seq (a + 1) b
+let rec iter f = function [] -> () | x :: l -> f x; iter f l
+let rec hash = function [] -> 0 | x :: l -> x + 7 * hash l
+
+type exn += Found
+
+let mem x l =
+  try iter (fun y -> if x = y then raise Found) l; false
+  with Found -> true
+
+let int_of_bool b = if b then 1 else 0
+
+let l = [1; 3; 7]
+
+let () = print_int (hash (map int_of_bool (map (fun x -> mem x l) (seq 0 5))))
