tests/expr01.ml
@@ -1,0 +1,42 @@
+let print n = print_int n; print_newline ()
+
+let () =
+  print 1;
+  print (- ( -2));
+  print (1 + 2);
+  print (let x = 2 in x + x);
+  print ((fun x -> x + 2) 3);
+  print (2 * 3);
+  print (2 * 3 + 1);
+  print (2 * (3 + 1));
+  print (95 / 10);
+  print (109 mod 11)
+
+let () =
+  (* TODO: max_int; abs; land, ^, int_of_char, etc  *)
+  for a = -10 to 10 do
+    print (succ a);
+    print (pred a);
+    for b = -10 to 10 do
+      print (a + b);
+      print (a * b);
+      print (a - b);
+      if b <> 0 then print (a / b);
+      if b <> 0 then print (a mod b);
+    done
+  done
+
+let () =
+  let f x = (x + 3) * (x / 2) + if x > 2 then 10 else 20 in
+  print (f 0 + f 1 + f 10)
+
+
+let f x = (x + 3) * (x / 2) + if x > 2 then 10 else 20
+
+let rec map f = function [] -> [] | x :: l -> f x :: map f l
+
+let rec sum = function [] -> 0 | x :: l -> x + sum l
+
+let rec seq a b = if a > b then [] else a :: seq (a + 1) b
+
+let () = print (sum (map f (seq 0 20)))
