tests/nondet01.ml
@@ -1,0 +1,29 @@
+let x =
+  let r = ref 0 in
+  assert (r := !r + 1; true);
+  !r
+
+let () = print_int x
+
+exception A
+exception B
+
+let () =
+  print_int (try raise A + raise B with A -> 1 | B -> 2);
+  ()
+
+
+(* ocamlc/opt print BA but the osiris interpreter prints AB
+-- probably because it did not choose the order
+indeed with:
+./interp.exe --detcheck nondet01.ml
+we can see that there are different possible outputs
+type s = { a : unit; b : unit }
+let _ = { a = print_string "A"; b = print_string "B" }
+*)
+
+
+(* ocamlc/opt print ABBA but the osiris interpreter prints BABA:
+let () = match (print_string "A", print_string "B") with _ -> ()
+let () = match (print_string "A", print_string "B") with _ -> () | exception _ -> ()
+*)
