tests/nondet02.ml
@@ -1,0 +1,152 @@
+(* from eval_order_xx.ml in ocaml's testsuite *)
+
+let ignore _ = ()
+let incr i = i := !i + 1
+module Fun = struct let id x = x end
+
+(* eval_order_1.ml *)
+
+let f x y = print_int x; print_int y
+
+let i = ref 0
+let () = f (incr i; !i) !i
+
+
+(* eval_order_2.ml *)
+
+(* PR#6136 *)
+
+exception Ok
+
+let first () =
+  let f g x = ignore (failwith "called f"); g in
+  let g x = x in
+  f g 2 (raise Ok)
+
+let second () =
+  let f g x = ignore (failwith "called f"); g in
+  let g x = x in
+  let h f = f g 2 (raise Ok) in
+  ignore (h f)
+
+let () =
+  try
+    ignore (first ());
+    assert false
+  with Ok ->
+    try
+      ignore (second ());
+      assert false
+    with Ok -> ()
+
+
+(* eval_order_3.ml *)
+
+let i = ref 0
+
+let f x y = print_int x; print_int y; 0
+[@@inline never]
+
+let foo _ = ()
+
+let foobar baz =
+  let incr_i _ =
+    incr i;
+    !i
+  in
+  let b = !i in
+  let z = foo 42 in
+  let a = (incr_i [@inlined never]) z in
+  let x = f a b in
+  x + 1
+
+let () =
+  ignore ((foobar 0) : int)
+
+(* eval_order_4.ml *)
+
+(* PR#7531 *)
+
+let f =
+  (let _i = print_endline "first"
+   in fun q -> fun i -> "") (print_endline "x")
+
+let _ =
+  let k =
+    (let _i = print_int 1
+     in fun q -> fun i -> "") ()
+  in k (print_int 0)
+
+let () =
+  print_endline "foo";
+  ignore ((f ()) : string);
+  ignore ((f ()) : string);
+  print_endline "bar"
+
+(* (no file eval_order_5.ml) *)
+
+(* eval_order_6.ml: unsupported: mutable record *)
+
+(* eval_order_7.ml *)
+
+let p i x =
+  print_int i;
+  print_newline ();
+  x
+
+let _ =
+  for i = (p 13 0) to (p 25 3) do
+    p i ()
+  done
+
+
+(* eval_order_8.ml *)
+
+(* closed, inlined *)
+let[@inline always] f () () = print_endline "4"
+let () = (let () = print_string "3" in f) (print_string "2") (print_string "1")
+
+(* closed, not inlined *)
+let[@inline never] f () () = print_endline "4"
+let () = (let () = print_string "3" in f) (print_string "2") (print_string "1")
+
+(* closure, inlined *)
+let[@inline never] g x =
+  (let () = print_string "3" in fun () () -> print_endline x)
+    (print_string "2") (print_string "1")
+let () = g "4"
+
+(* closure, not inlined *)
+let[@inline never] g x =
+  (let () = print_string "3" in
+   let[@inline never] f () () = print_endline x in f)
+    (print_string "2") (print_string "1")
+let () = g "4"
+
+(* eval_order_9.ml *)
+
+(* From #12440, by Jeremy Yallop --> this one fails on ocamlopt, in fact *)
+(*
+let _ =
+  let r = ref true in
+  match Fun.id ((r := false), !r) with
+  | _, true  -> print_endline "Ok"
+  | _, false -> print_endline "ERROR"
+*)
+
+
+(* eval_order_pr10283.ml *)
+
+(* Slightly modified version of an example from github user @Ngoguey42,
+   submitted as issue number 10283. *)
+
+let[@inline never][@local never] g () =
+  let[@local always] f a b = print_int a; print_int b in
+
+  let i = ref 0 in
+  f (incr i; !i) (incr i; !i)
+
+let () = g ()
+
+(* float_physical_equality.ml -- unsupported *)
+(* float.ml -- unsupported *)
