coq-osiris/theories/program_logic/ewp.v
@@ -114,7 +114,7 @@ Definition is_handleable {A X} (m : micro A X) : option handleable :=
   match m with
   | Ret v => Some (HRet v)
   | Throw e => Some (HThrow e)
-  | Crash => Some HCrash
+  | Crash _ => Some HCrash
   | Stop CPerf e k => Some (HPerform e k)
   | _ => None
   end.
