tests/runtests.sh
@@ -1,0 +1,16 @@
+#!/bin/bash
+set -euo pipefail
+
+# This tests that the osiris interpreter produces the same output as ocaml on
+# each of the test files
+
+time for f in *.ml
+do
+    test=${f%.ml}
+    echo -ne "test: $test\t"
+    ./interp.exe $test.ml > $test.olang
+    rm -f $test.ml.cmi # TODO make this unnecessary then remove
+    ocaml $test.ml > $test.ocaml
+    diff $test.ocaml $test.olang && echo ok || echo NOK
+    rm -f $test.ocaml $test.olang
+done
